lib/Lib.IntVector.fsti
@@ -206,8 +206,12 @@ val vec_rotate_right_lemma: #t:v_inttype -> #w:width
 
 inline_for_extraction noextract
 val vec_rotate_left: #t:v_inttype -> #w:width
+  -> v1:vec_t t w -> s:rotval t{t <> U128 \/ uint_v s % 8 == 0} -> vec_t t w
+
+val vec_rotate_left_lemma: #t:v_inttype -> #w:width
   -> v1:vec_t t w -> s:rotval t{t <> U128 \/ uint_v s % 8 == 0} ->
-  v2:vec_t t w{vec_v v2 == map (rotate_left_i s) (vec_v v1)}
+ Lemma (ensures (vec_v (vec_rotate_left v1 s) == map (rotate_left_i s) (vec_v v1)))
+ [SMTPat (vec_v (vec_rotate_left v1 s))]
 
 inline_for_extraction noextract
 val vec_eq_mask: #t:v_inttype -> #w:width -> v1:vec_t t w -> v2:vec_t t w -> v3:vec_t t w{vec_v v3 == map2 eq_mask (vec_v v1) (vec_v v2)}
